theories/Data/FiniteMap.v
@@ -1,14 +1,17 @@
 Require Import PnV.Prelude.Prelude.
 Require Import PnV.Prelude.X.
+Require Import PnV.Data.FiniteSet.
 
 #[local] Infix "=~=" := is_similar_to : type_scope.
 #[local] Infix "∈" := L.In.
 
 Module FM.
 
+Import FS.
+
 #[universes(template), projections(primitive)]
 Record alist {K : Type} {V : Type} : Type :=
-  mk_alist { kvlist : list (K * V) } as al.
+  mk_alist { kvlist : fin_ensemble (K * V) } as al.
 
 #[global] Arguments alist : clear implicits.
 
